Chore: Add simple nameless STLC proofs

theories/Semantics.v
@@ -1,7 +1,7 @@
 From MetaCoq.Erasure.Typed Require Import ExAst Utils WcbvEvalAux.
 From MetaCoq.Erasure.Typed Require Import TypeAnnotations.
 From MetaCoq.Erasure.Typed Require Import Annotations.
-From MetaCoq.Erasure Require Import EAst ECSubst EWellformed.
+From MetaCoq.Erasure Require Import EAst ECSubst ELiftSubst EWellformed.
 From MetaCoq.Utils Require Import utils.
 
 From VTL Require Import PIR BigStepPIR Translation.
@@ -24,27 +24,37 @@ Inductive InSubset (ctx : list bs) : EAst.term -> Prop :=
   | S_tRel : forall n res,
     nth_error ctx n = Some res ->
     InSubset ctx (tRel n)
-  | S_tLambda : forall na b,
-    InSubset ctx b ->
-    InSubset ctx (tLambda na b)
+  | S_tLambda : forall x b,
+    InSubset (x :: ctx) b ->
+    InSubset ctx (tLambda (BasicAst.nNamed x) b)
   | S_tApp : forall t1 t2,
     InSubset ctx t1 ->
     InSubset ctx t2 ->
     InSubset ctx (tApp t1 t2)
 .
 
+Lemma sub_ctx_ext : forall ctx x t,
+  InSubset ctx t ->
+  InSubset (x :: ctx) t.
+Proof.
+  intros ctx x t sub.
+  induction sub.
+  - constructor.
+  - simpl. admit.
+  - constructor. admit.
+  - simpl. constructor. apply IHsub1. apply IHsub2.
+Admitted.
+
 Import Coq.Strings.String.
 Local Open Scope string_scope.
 Import MCMonadNotation.
 
-Notation "ctx ⊢ tl{ gt | ann_gt }" := (translate_term remap_env ctx gt ann_gt) (at level 100).
 Notation "pt '⇓ₚ' pv" :=
   (evaluatesTo pt pv)
   (at level 50).
 
 Ltac solve_pir_eval := split; [(eexists ; eauto using eval) | constructor].
-Ltac solve_inv := intros pt pv Hgt Hgv; inversion Hgt; inversion Hgv; solve_pir_eval.
-Ltac solve_err := simpl in *; try contradiction; try discriminate.
+Ltac tl_reflect H := apply translate_reflect in H.
 
 Definition gal_id :=
   tLambda (BasicAst.nNamed "x"%bs) (tRel 0).
@@ -66,11 +76,8 @@ Theorem id_correct_implicit : forall Σ ctx (ann : annots box_type gal_id) pir_i
   pir_id ⇓ₚ pir_id.
 Proof with (eauto using eval).
   intros Σ ctx ann pir_id ev tl.
-  unfold gal_id in *.
-  destruct ann as [ty t_ty]. rewrite unfold_lamAbs in tl.
-  destruct ty; try discriminate.
-  destruct (translate_ty remap_env ty1);
-  inversion tl; solve_pir_eval.
+  tl_reflect tl.
+  inversion tl. solve_pir_eval.
 Qed.
 
 (* contexts don't match in both branches! *)
@@ -82,12 +89,10 @@ Lemma tl_app : forall ctx t1 t2 ann_t (t' : PIR.term),
     Apply t1' t2' = t'.
 Proof.
   intros ctx t1 t2 ann_t t' tl_a.
-  inversion tl_a as [Ha].
-  destruct ann_t as [ann_t [ann_t1 ann_t2]].
-  destruct (translate_term remap_env ctx t1 ann_t1) as [t1'|] eqn:Et1; try discriminate.
-  destruct (translate_term remap_env ctx t2 ann_t2) as [t2'|] eqn:Et2; try discriminate. 
-  simpl in Ha. exists ann_t1. exists ann_t2. exists t1'. exists t2'.
-  inversion Ha. auto.
+  tl_reflect tl_a.
+  inversion tl_a.
+  exists ann_t1. exists ann_t2. exists t1'. exists t2'.
+  tl_reflect H1. tl_reflect H4. auto.
 Qed.
   
 Theorem refl_tl_correct : forall Σ ctx gt (ann : annots box_type gt) pt,
@@ -101,42 +106,76 @@ Proof with (eauto using eval).
   - (* TBox *) inversion tl. solve_pir_eval.
   - (* tRel, either a translation error or ev is invalid *) 
     now inversion ev.
-  - (* tLambda *) destruct ann as [ty t_ty]; try discriminate. 
-    destruct na.
-    + solve_err. 
-    + simpl in tl. destruct ty; try discriminate.
-      destruct (translate_ty remap_env ty1) as [ty1'|]; try discriminate.
-      destruct (i :: ctx ⊢ tl{ b | t_ty}) as [b'|]; try discriminate.
-      inversion tl. solve_pir_eval.
+  - (* tLambda *) tl_reflect tl. 
+    inversion tl. solve_pir_eval.
 Qed.
-
-(* subst lemma, or use the named variant of EAst *)
-(* Print csubst. *)
-Lemma tl_subst : forall ctx k x v b ann_v ann_b ann_t v' b',
-  translatesTo remap_env ctx v ann_v v' ->
-  translatesTo remap_env ctx b ann_b b' ->
-  translatesTo remap_env ctx (csubst v k b) ann_t (BigStepPIR.subst x v' b').
-Proof.
-  intros ctx k x v b ann_v ann_b ann_t v' b' tlt_v tlt_b.
-  inversion tlt_b.
-  - simpl. subst. apply tlt_tt.
-  - simpl in *. destruct (x =? (bs_to_s x0)). subst.
-    simpl in *. inversion tlt_v. Admitted.
-
 
 Definition id_app := tApp
   (tLambda (BasicAst.nNamed "x"%bs) (tRel 0)) (tBox).
 
+Print ELiftSubst.subst.
+Print csubst.
+Print annots.
+Print tLambda.
+
+Print gal_id.
+Eval cbv in csubst 
+  (tLambda (BasicAst.nNamed "y"%bs) (tRel 0))
+  0
+  gal_id.
+Eval cbv in (tLambda (BasicAst.nNamed "x"%bs (tLambda (BasicAst.nNamed "y"))))
+
+Print eval.
+Lemma tl_subst : forall ctx k x v b ann_v ann_b ann_t v' b',
+  (* closed  *)
+  (* nth_error ctx k = Some x -> *)
+  translatesTo remap_env ctx v ann_v v' ->
+  translatesTo remap_env ctx b ann_b b' ->
+  translatesTo remap_env ctx (csubst v k b) ann_t (BigStepPIR.subst x v' b').
+Proof.
+  intros ctx k x v b ann_v ann_b ann_t v' b'. revert ctx k ann_t b'.
+  induction b; intros ctx k' ann_t b' tlt_v tlt_b; inversion tlt_b.
+  - apply tlt_tt.
+  (* - destruct (k' =? n)%nat eqn:Enk.
+    rewrite Nat.eqb_eq in Enk. *)
+  - simpl in *. destruct (x =? (bs_to_s x0)).
+    + destruct (k' ?= n)%nat eqn:ekn.
+      * admit. (* ann_t must be ann_v, how to prove this *)
+      * admit.
+      * admit.
+    + destruct (k' ?= n)%nat eqn:ekn.
+      * admit.
+      * admit.
+      * subst. admit.
+  - destruct ann_t as [ty ann_sb].
+    simpl in *. destruct (x =? (bs_to_s x0)).
+    + admit.
+    + admit.
+  - simpl in *.
+    destruct ann_t as [t_ty [ann_st1 ann_st2]].
+    specialize (IHb1 ann_t1 ctx k' ann_st1 t1' tlt_v H1).
+    specialize (IHb2 ann_t2 ctx k' ann_st2 t2' tlt_v H4).
+    apply (tlt_app remap_env ctx). apply IHb1. apply IHb2.
+Admitted.
+
+(* lemma for general and closed *)
 Theorem stlc_correct : forall Σ ctx 
-  gt (ann_gt : annots box_type gt) pt
-  gv (ann_gv : annots box_type gv) pv,
-  Σ e⊢ gt ⇓ gv ->
-  InSubset ctx gt ->
-  translate_term remap_env ctx gt ann_gt = Some pt ->
-  InSubset ctx gv ->
-  translate_term remap_env ctx gv ann_gv = Some pv ->
-  pt ⇓ₚ pv.
+  t (ann_t : annots box_type t) t'
+  v (ann_v : annots box_type v),
+  [] e⊢ t ⇓ v ->
+  InSubset nil t ->
+  translatesTo remap_env ctx t ann_t t' ->
+  exists ann_v v' k,
+    translatesTo remap_env ctx v ann_v v' /\
+    eval t' v' k.
 Proof with (eauto using eval).
-  intros Σ ctx gt ann_gt pt gv ann_gv pv ev sub_gt.
-  revert pt pv. induction ev; try discriminate; intros pt pv.
-  - simpl. destruct ann_gt. Admitted.
+  intros Σ ctx t ann_t t' v ann_v ev. revert t'.
+  induction ev; intros t'' sub tlt_t; inversion sub.
+  - admit.
+  - inv tlt_t.
+    admit.
+  - admit.
+  - admit.
+  - Admitted.
+  
+  
